src/HOL/MicroJava/J/Exceptions.thy
@@ -10,9 +10,9 @@ definition blank :: "'c prog \<Rightarrow> cname \<Rightarrow> obj" where
   "blank G C \<equiv> (C,init_vars (fields(G,C)))" 
 
 definition start_heap :: "'c prog \<Rightarrow> aheap" where
-  "start_heap G \<equiv> Map.empty (XcptRef NullPointer \<mapsto> blank G (Xcpt NullPointer))
-                        (XcptRef ClassCast \<mapsto> blank G (Xcpt ClassCast))
-                        (XcptRef OutOfMemory \<mapsto> blank G (Xcpt OutOfMemory))"
+  "start_heap G \<equiv> Map.empty (XcptRef NullPointer \<mapsto> blank G (Xcpt NullPointer),
+                        XcptRef ClassCast \<mapsto> blank G (Xcpt ClassCast),
+                        XcptRef OutOfMemory \<mapsto> blank G (Xcpt OutOfMemory))"
 
 
 abbreviation
